light rework at certificate and CKTInput

CKTInput.dfy
@@ -7,7 +7,7 @@ predicate isInputCKT (input:seq<string>)
 }
 predicate isStringAGate(str:string)
 {
-    str=="AND" || str=="OR" || str=="NOR"
+    str=="AND" || str=="OR" || str=="NOT"
 }
 predicate isAGoodPozInput(nr:string,poz:nat)
     requires isStringAValidNumber(nr)
@@ -22,20 +22,20 @@ predicate isStringAValidPos(input:seq<string>, pos:nat)
     requires pos<|input|
     requires isStringAValidNumber(input[pos])
 {
-    pos-1-stringToNat(input[pos])>=0 && !isStringAValidNumber(input[pos-1-stringToNat(input[pos])])
+    0<=stringToNat(input[pos])<pos && !isStringAValidNumber(input[stringToNat(input[pos])])
 }
-predicate isInputCKT' (input:seq<string>, pos:nat)
+predicate isInputCKT' (input:seq<string>, pos:nat) // nu mai ai nume custom pentru variabile
     requires pos<|input|
 {
     match input[pos]
         case "AND" => 2<pos<|input| && isStringAValidNumber(input[pos-1]) && isStringAValidPos(input, pos-1) && isStringAValidNumber(input[pos-2]) && isStringAValidPos(input, pos-2)
         case "OR" => 2<pos<|input| && isStringAValidNumber(input[pos-1]) && isStringAValidPos(input, pos-1) && isStringAValidNumber(input[pos-2]) && isStringAValidPos(input, pos-2)
         case "NOT" => 1<pos<|input|&& isStringAValidNumber(input[pos-1]) && isStringAValidPos(input, pos-1) 
-        case x => if isStringAValidNumber(x) then isStringAValidPos(input, pos)
-                    else !(x in ReservedWords)
+        case "VARIABLE" => true
+        case x => false 
 }
 
- lemma Lemma_ValidInputExtension(input: seq<string>, ext: seq<string>)
+ lemma ValidInputExtension(input: seq<string>, ext: seq<string>)
     requires isInputCKT(input)
     requires forall k :: |input| <= k <|input|+ |ext| ==> isInputCKT'(input + ext, k)
     ensures isInputCKT(input + ext)
@@ -45,20 +45,58 @@ predicate isInputCKT' (input:seq<string>, pos:nat)
     assert forall i :: 0 <= i < |input| ==> isInputCKT'(input, i);
     assert forall i :: 0 <= i < |input| && isInputCKT'(input,i)==> isInputCKT'(combined, i);
 }
+function nthVariableInput (input:seq<string>, pos:nat) : nat
+    requires pos<|input|
+    requires input[pos]=="VARIABLE"
+{
+    nthVariableInput'(input,0,pos)
+}
+function nthVariableInput'(input:seq<string>,initPos:nat, pos:nat) :nat 
+    requires initPos<=pos
+    requires pos<|input|
+    requires input[pos]=="VARIABLE"
+    ensures initPos<pos && input[initPos]=="VARIABLE" ==> nthVariableInput'(input,initPos,pos)==nthVariableInput'(input,initPos+1,pos)+1
+    ensures initPos<pos ==> nthVariableInput'(input,initPos,pos)>=nthVariableInput'(input,initPos+1,pos)
+    decreases pos-initPos
+{
+    if initPos==pos then 
+        0
+    else
+        if input[initPos]=="VARIABLE" then
+           nthVariableInput'(input,initPos+1,pos)+1
+        else
+            nthVariableInput'(input,initPos+1,pos)
+}
+lemma nthVariableInputIsUnique (input:seq<string>, pos1:nat,pos2:nat)
+    requires pos1<pos2<|input|
+    requires input[pos1]=="VARIABLE" && input[pos2]=="VARIABLE"
+    ensures nthVariableInput(input,pos1)<nthVariableInput(input,pos2)
+{
+    assert nthVariableInput(input,pos1)==nthVariableInput'(input,0,pos1);
+    assert nthVariableInput(input,pos2)==nthVariableInput'(input,0,pos2);
+    assert nthVariableInput'(input,pos1,pos2)>nthVariableInput'(input,pos1,pos1);
+    if pos1>0 {
+        for k:=pos1-1 downto 0
+            invariant nthVariableInput'(input,k,pos2)>nthVariableInput'(input,k,pos1)
+        {
+        }
+    }
+    assert nthVariableInput'(input,0,pos2)>nthVariableInput'(input,0,pos1);
+}
+
 predicate isCertificateValidForInput (input:seq<string>,k:seq<string>)
     requires isCertificateCorrectForm(k)
 {
-    forall pos:nat:: pos<|input| ==> if !(input[pos] in ReservedWords) && !isStringAValidNumber(input[pos]) then (input[pos] in k) else true
+    forall pos:nat:: pos<|input| && input[pos]=="VARIABLE" ==> nthVariableInput(input,pos)<|k|
 }
 ghost predicate isLanguageCKT(l:Language)
 {
-    forall input:seq<string> :: (input in l) <==> exists pos:nat:: 1<=pos<|input|-3 
-                                            && isInputCKT(input) 
+    forall input:seq<string> :: (input in l) <==> isInputCKT(input) 
 }
 ghost predicate isInputSymbolsValidForLanguage(l:Language,inputS:InputSymbols)
 {
     forall input:seq<string>::  input in l <==> 
-                                exists c:seq<string> :: isInputValid(input+c,inputS)
+                                exists c:seq<string>,k:certificate :: isCertificateCorrectForm(k) && isInputValid(input+k,inputS)
 }
 ghost predicate inputSymbolsForCKT (inputS:InputSymbols,l:Language)
     requires isLanguageCKT(l)
@@ -71,9 +109,3 @@ ghost predicate AdditionalTapeSymbolsForCKT(inputS:InputSymbols,l:Language,addTa
 {
     isTapeSymbolsValid(inputS,addTapeS)
 }
-// lemma isCKTNP (l:Language)
-// requires isLanguageCKT(l)
-// ensures isLanguageNPTIME2(l)
-// {
-
-// }
