Certificate.dfy
@@ -3,31 +3,12 @@ include "turing_machine.dfy"
 type certificate=seq<string>
  predicate isCertificateCorrectForm (k:certificate)
 {
-    (|k|>0 && |k|%2==0) && (forall pos:nat:: pos<|k| ==> (if pos%2==1 then 
-    (k[pos]!="TRUE" && k[pos]!="FALSE") 
-    else (k[pos]=="TRUE" || k[pos]=="FALSE"))) 
+    forall pos:nat:: pos<|k| ==> (k[pos]=="TRUE" || k[pos]=="FALSE")
 }
- function findValue(k:certificate,v:string) : Option<bool>
+ function findValue(k:certificate,pos:nat) : bool
     requires isCertificateCorrectForm(k)
-    requires v!="TRUE" && v!="FALSE"
+    requires pos<|k|
  {
-    findValue'(k,v,1)
- }
- function findValue'(k:certificate,v:string,pos:nat): Option<bool>
-    requires 0<pos<=|k|
-    requires isCertificateCorrectForm(k)
-    requires v!="TRUE" && v!="FALSE"
-    decreases |k|-pos
-
- {
-    if pos==|k| then 
-        None
-    else
-        if k[pos]==v then
-            if k[pos-1]=="TRUE" then 
-                Some(true)
-            else
-                Some(false)
-        else
-            findValue'(k,v,pos+1)
+    if k[pos]=="TRUE" then true
+    else false 
  }
