Circuit.dfy
@@ -19,12 +19,6 @@ predicate isAGoodPoz (e:circuitCell,poz:nat)
         case POZ(nr) => (
             0<=nr<=poz-1)
 }
-predicate isAGoodVariableCircuit(e:circuitCell)
-    requires isCircuitCellAVariable(e)
-{
-    match e 
-        case VARIABLE(x) => !isStringAValidNumber(x) && !(x in ReservedWords)
-}
 predicate isCircuitGood(c:circuit)
 {
     forall poz:nat::poz<|c| ==> isCircuitGood'(c[poz],poz)
@@ -35,9 +29,7 @@ predicate isCircuitGood'(c:circuitCell,poz:nat)
     if isCircuitCellAPoz(c) then
         isAGoodPoz(c,poz)
     else
-        if isCircuitCellAVariable(c) then 
-            isAGoodVariableCircuit(c)
-        else true 
+        true 
 }
 predicate isCircuitValid (c:circuit)
 {
@@ -50,28 +42,73 @@ predicate isCircuitValid'(c:circuit, pos:nat)
             case AND => 2<pos<|c| && isCircuitCellAPoz(c[pos-1]) && isCircuitCellAPoz(c[pos-2])
             case OR => 2<pos<|c|  && isCircuitCellAPoz(c[pos-1]) && isCircuitCellAPoz(c[pos-2])
             case NOT => 1<pos<|c| && isCircuitCellAPoz(c[pos-1]) 
-            case VARIABLE (x) => isAGoodVariableCircuit(c[pos])
+            case VARIABLE (x) => true // numele variabilei va fi pierduta in traducere
             case POZ(nr) => isAGoodPoz(c[pos],pos) && !isCircuitCellAPoz(c[nr])
 }
-// predicate isThatPOZValid(c:circuit,pos:nat)
-//     requires pos<|c|
-// {
-//     match c[pos]
-//          case POZ(nr) =>  pos>0 && 0<nr<pos-1 && pos-nr-1>=0 && !isCircuitCellAPoz(c[nr])
-//          case _=>true
-// }
+predicate isThatPOZValid(c:circuit,pos:nat)
+    requires pos<|c|
+{
+    match c[pos]
+         case POZ(nr) =>  pos>0 && 0<nr<pos-1 && pos-nr-1>=0 && !isCircuitCellAPoz(c[nr])
+         case _=>true
+}
+function nthVariableCircuit (c:circuit, pos:nat) : nat
+    requires pos<|c|
+    requires isCircuitCellAVariable(c[pos])
+{
+    nthVariableCircuit'(c,0,pos)
+}
+function nthVariableCircuit'(c:circuit,initPos:nat,pos:nat) :nat 
+    requires initPos<=pos
+    requires pos<|c|
+    requires isCircuitCellAVariable(c[pos])
+    ensures initPos<pos && isCircuitCellAVariable(c[initPos]) ==> nthVariableCircuit'(c,initPos,pos)==nthVariableCircuit'(c,initPos+1,pos)+1
+    ensures initPos<pos ==> nthVariableCircuit'(c,initPos,pos)>=nthVariableCircuit'(c,initPos+1,pos)
+    decreases pos-initPos
+{
+    if initPos==pos then 
+        0
+    else
+        if isCircuitCellAVariable(c[initPos]) then
+            nthVariableCircuit'(c,initPos+1,pos)+1
+        else
+            nthVariableCircuit'(c,initPos+1,pos)
+}
+lemma nthVariableCircuitIsUnique (c:circuit, pos1:nat,pos2:nat)
+    requires pos1<pos2<|c|
+    requires isCircuitCellAVariable(c[pos1]) && isCircuitCellAVariable(c[pos2])
+    ensures nthVariableCircuit(c,pos1)<nthVariableCircuit(c,pos2)
+{
+    assert nthVariableCircuit(c,pos1)==nthVariableCircuit'(c,0,pos1);
+    assert nthVariableCircuit(c,pos2)==nthVariableCircuit'(c,0,pos2);
+    assert nthVariableCircuit'(c,pos1,pos2)>nthVariableCircuit'(c,pos1,pos1);
+    if pos1>0 {
+        for k:=pos1-1 downto 0
+            invariant nthVariableCircuit'(c,k,pos2)>nthVariableCircuit'(c,k,pos1)
+        {
+        }
+    }
+    assert nthVariableCircuit'(c,0,pos2)>nthVariableCircuit'(c,0,pos1);
+}
 
-predicate isCertificateValid (c:circuit,k:certificate)
+predicate isCertificateValidForCircuit (c:circuit,k:certificate)
     requires isCertificateCorrectForm(k)
     requires isCircuitValid(c)
 {
-     forall pos:nat:: pos<|c| ==> match c[pos]
-                                    case VARIABLE(x) => 
-                                    assert isCircuitValid'(c,pos);
-                                    assert !(x in ReservedWords);
-                                    findValue(k,x)!=None
-                                    case _ => true
- }
+    forall pos:nat:: pos<|c| && isCircuitCellAVariable(c[pos]) ==> nthVariableCircuit(c,pos)<|k|
+}
+function getValueFromCertificate(c:circuit,pos:nat,k:certificate) : bool
+    requires isCertificateCorrectForm(k)
+    requires isCircuitValid(c)
+    requires isCertificateValidForCircuit(c,k)
+    requires pos<|c|
+    requires isCircuitCellAVariable(c[pos])
+{
+    if k[nthVariableCircuit(c,pos)]=="TRUE" then
+        true
+    else 
+        false
+}
  lemma Lemma_ValidCircuitExtension(c: circuit, ext: seq<circuitCell>)
     requires isCircuitValid(c)
     requires forall k :: |c| <= k <|c|+ |ext| ==> isCircuitValid'(c + ext, k)
@@ -84,59 +121,18 @@ predicate isCertificateValid (c:circuit,k:certificate)
     assert forall i :: 0 <= i < |c| && isCircuitValid'(c,i)==> isCircuitValid'(combined, i);
     assert isCircuitValid(combined);
 }
- predicate variableHasValue(c:circuit,k:certificate,pos:nat)
-    requires pos<|c|
- {
-    match c[pos] 
-                 case VARIABLE(x) => exists poz:nat :: (1<poz<|k| && (
-                     k[poz]==x && (k[poz-1]=="TRUE" && k[poz-1]=="FALSE"))) 
-                 case _ => true
- }
-function getValueFromCertificate (v:string,k:certificate):Option<bool>
-     requires v!="FALSE" && v!="TRUE"
-     requires isCertificateCorrectForm (k)
-
-{
-    getValueFromCertificate'(v,k,0)
-}
-function getValueFromCertificate'(v:string,k:certificate,pos:nat):Option<bool>
-    requires pos<=|k|
-    requires v!="FALSE" && v!="TRUE"
-    decreases |k|-pos
-    ensures getValueFromCertificate'(v,k,pos)!=None <==>exists poz:nat :: (0<poz<|k| && (
-                    k[poz]==v && (k[poz-1]=="TRUE" || k[poz-1]=="FALSE")))
-    requires forall poz:nat ::poz<pos ==> k[poz]!=v
-    ensures forall poz:nat ::poz<pos ==>  k[poz]!=v
-    requires isCertificateCorrectForm(k)
-
-{
-    if pos==|k| then None
-    else
-        if k[pos]==v then(
-            assert  v!="FALSE" && v!="TRUE";
-            assert k[pos]!="TRUE" && k[pos]!="FALSE";
-            assert k[pos-1]=="TRUE" || k[pos-1]=="FALSE";
-            if k[pos-1]=="TRUE" then 
-                Some(true)
-            else
-                Some(false)
-            )
-        else
-            getValueFromCertificate'(v,k,pos+1)
-}
 predicate solveCircuit(c:circuit,k:certificate)
     requires isCircuitValid(c)
     requires isCertificateCorrectForm(k)
-    requires isCertificateValid(c,k)
+    requires isCertificateValidForCircuit(c,k)
     requires |c|>=1
 {
     solveCircuit'(c,k,|c|-1)
 }
 predicate solveCircuit'(c:circuit,k:certificate,pos:nat)
     requires isCircuitValid(c)
-    requires |k|>=1 && |k|%2==0
     requires isCertificateCorrectForm(k)
-    requires isCertificateValid(c,k)
+    requires isCertificateValidForCircuit(c,k)
     requires |c|>=1
     requires pos<|c|
     decreases pos
@@ -152,17 +148,13 @@ predicate solveCircuit'(c:circuit,k:certificate,pos:nat)
         case NOT  =>
             assert  isCircuitValid'(c, pos);        
         !solveCircuit'(c,k,pos-1)
-        case VARIABLE (x) =>( assert isCircuitValid'(c,pos);     
-            match findValue(k,x)
-                                        case Some(st) => st
-                                        case None => false )
+        case VARIABLE (x) => getValueFromCertificate(c,pos,k)
         case POZ(nr)=>
             assert  isCircuitValid'(c, pos);
             solveCircuit'(c,k,nr)
 }
-
 ghost predicate checkSatisfaction(c:circuit)
     requires isCircuitValid(c)
 {
-    exists k:certificate :: isCertificateCorrectForm(k) && isCertificateValid(c,k) && |c|>=1 && solveCircuit(c,k)
+    exists k:certificate :: isCertificateCorrectForm(k) && isCertificateValidForCircuit(c,k) && |c|>=1 && solveCircuit(c,k)
 }
